%%This is a very basic article template.
%%There is just one section and two subsections.
\documentclass{article}

\usepackage{fullpage}
\usepackage[parfill]{parskip}
\usepackage{amsmath}
\usepackage{amssymb}

\title{PMATH 345 - Assignment 1}
\author{Adrian Petrescu (\#20240298)}

\begin{document}

\maketitle

\textbf{1. (a) Let $R = \mathbb{R}[x, y]$ be the set of all polynomials in two
variables with real coefficients. Let $S$ be the subset of polynomials $p(x, y)$ such that
$p_x(0, 0) = 0$ ($p_x$ denotes the partial derivative of $p$ with respect to
$x$). Is $S$ a subring of $R$? Prove your answer.}

To check if $S$ is a subring, three things need to be checked. 

The additive identity for $R$ is the zero polynomial $p(x,y)=0$, whose partial
derivative with respect to $x$ is also the zero polynomial, which is $0$ at the origin,
and therefore in $S$. Similarly, the multiplicative inverse $p(x,y)=1$ has the
same partial derivative with respect to $x$, so it is also in $S$.

Next, we check that $S$ is closed under subtraction. Let $p(x,y),q(x,y)\in S$.
We want to check if $r(x,y)=p(x,y)-q(x,y)$ is also in $S$. It is obvious that
$r$ is a polynomial, but it remains to show that $r_x(0,0)=0$. Well,
polynomials are smooth, so we can safely use the subtraction rule for partial
derivatives. That is,
\begin{align*}
	&\frac{\partial{r}}{\partial{x}}=\frac{\partial}{\partial{x}}(p-q)=\frac{\partial p}{\partial x} - \frac{\partial q}{\partial x} \\
	\implies&r_x(x,y)=p_x(x,y)-q_x(x,y) \\
	\implies&r_x(0,0)=p_x(0,0)-q_x(0,0)=0 \\
	\implies&r\in S
\end{align*}

Lastly, we check that $S$ is closed under multiplication. Let $s(x,y)=p(x,y)q(x,y)$. Once again we can use the product rule 
for partial derivatives, so
\begin{align*}
	&\frac{\partial{r}}{\partial{x}} = q\frac{\partial p}{\partial{x}} +
	p\frac{\partial{q}}{\partial{x}} \\
	\implies &s_x(x,y) = p_x(x,y)q(x,y) + p(x,y)q_x(x,y) \\
	\implies &s_x(0,0) = 0 \\
	\implies &s\in S
\end{align*}

Thus, by the subring theorem, $S$ is a subring of $R$.

\textbf{(b) Let $R = \mathbb C$, the set of complex numbers, and let $S$ be the
subset of complex numbers $z$ of the form $z = a + b\sqrt2$, where $a, b \in
\mathbb Z$ are integers. Is $S$ a subring of $R$? Prove your answer.}

Once more, we check the three facts. The multiplicative and additive identities
for $R$ are $1+0i=1+0\sqrt2\in S$ and $0+0i=0+0\sqrt2\in S$ respectively, so
the first condition is satisfied.

Next we check that $S$ is closed under subtraction:
\begin{align*}
	(a+b\sqrt2)-(c+d\sqrt2)=(a-c)+(b-d)\sqrt2\in S \quad\text{(Since the integers
	are a ring.)}
\end{align*}
Lastly, we check closure under multiplication:
\begin{align*}
	(a+b\sqrt2)(c+d\sqrt2)=&ac+ad\sqrt2+bc\sqrt2+2bd \\
	=&(ac+2bd) + (ad+bc)\sqrt2\in S
\end{align*}
So by the subring theorem, $S$ is a subring.

\textbf{2. (a) Is the mapping from $\mathbb Z_{10}$ to $\mathbb Z_{10}$ given by
$x\to2x$ a ring homomorphism? Prove your answer.}

This mapping fails the simplest condition for a homorphism. Simply, the
multiplicative identity of $\mathbb Z_{10}$ is $1$, which should be preserved
under a homomorphism, but under this mapping, it goes to $2$ which is not the
identity for $\mathbb Z_{10}$. Indeed, any homomorphism from a ring to itself
would have to have a fixed point at $1$ since the identity is unique, but the
only element with $x=2x$ is $x=0$, so the only ring under which this could be a
homomorphism would have to have $0$ as both the additive and multiplicative
identities: that is, the zero ring.

\textbf{(b) Let $\phi:\mathbb C[x]\to\mathbb C[x]$ be defined by
$\phi(p(x)) = p(x^2)$. Is $\phi$ a homomorphism? Prove your answer.}

We check the three properties of a homomorphism. First, the $0$ and $1$ of
$\mathbb C[x]$ are $p(x)=0$ and $p(x)=1$ respectively, neither of which are
affected by $\phi$, since they are constant polynomials, so it is true that
$\phi(1)=1$.

Next, consider $p(x)=\sum_{i=0}^n{a_ix^i}$ and $q(x)=\sum_{j=0}^m{b_jx^j}$.
Then we have:
\begin{align*}
&r(x)=p(x)+q(x)
\implies \phi(r)=r(x^2)=p(x^2)+q(x^2)=\phi(p)+\phi(q)
\end{align*}
Similarly,
\begin{align*}
s(x)=p(x)q(x)\implies\phi(s)=p(x^2)q(x^2)=\phi(p)\phi(q)
\end{align*}
So it satisfies the rules for addition and multiplication, and therefore is a
homomorphism.

\textbf{3. Let $\phi:\mathbb Z_9\to\mathbb Z_3$ be a homomorphism. What is
$\phi(4)$?}

By the definition of a homomorphism, $\phi(1)=1$. Also by the definition of a
homomorphism, $\phi(p_1+p_2)=\phi{(p_1)}+\phi{(p_2)}$. Putting these two facts
together, we get
\begin{align*}
\phi(4)=&\phi(1)+\phi(1)+\phi(1)+\phi(1) \\
	=& [1]_3+[1]_3+[1]_3+[1]_3 \\
	=& [4]_3=1
\end{align*}

\textbf{4. Let $R$ be a commutative ring, and let $\phi:R\to R$ be a
homomorphism. Define the following subset of $R$: \[ R^\phi=\{x\in
R\mid\phi(x)=x\} \] Is $R^\phi$ a subring of $R$? If so, prove your answer. If
not, give a specific example of a ring $R$ and a homomorphism $\phi:R\to R$
such that $R^\phi$ is not a ring.}

Firstly, it is clear (by definition) that $\phi(1)=1\implies 1\in R^\phi$. It
also follows easily from the fact that $\phi(0\cdot a)=\phi(0)\phi(a)=\phi(0)$
for any $a\in R$, that $\phi(0)=0\implies 0\in R^\phi$. So it only remains to
show that $R^\phi$ is closed under subtraction and multiplication.

Take $r_1,r_2\in R^\phi$. We want to see if $r_1r_2$ is in $R^\phi$; well,
$\phi(r_1r_2)=\phi(r_1)\phi(r_2)=r_1r_2$, so it is in $R^\phi$.

To show that $R^\phi$ is also closed under subtraction, we first show that
$-1\in R^\phi$. We know that $\phi(1+(-1))=\phi(1)+\phi(-1)$, but since we
already have that $\phi(1)=1$ and $\phi(0)=0$, it follows that $1+\phi(-1)=0$
which implies $\phi(-1)=-1$, so $(-1)\in R^\phi$. Now, using the result of
$5(a)$, we simply have
\begin{align*}
	\phi(r_1-r_2)=&\phi(r_1+(-1)(r_2))=\phi(r_1)+\phi(-1)\phi(r_2)\\
	=&r_1+(-1)r_2=r_1-r_2\implies(r_1-r_2)\in R^\phi
\end{align*}
Thus, $R^\phi$ is a subring of $R$.

\textbf{5. Let $R$ be a commutative ring.}

\textbf{(a) Prove that $-x=(-1)x$ for all $x\in R$. (Recall that $-x$ denotes
the additive inverse of $x$, and $(-1)x$ denotes the product of $x$ with $-1$,
the additive inverse of $1$.)}

We wish to prove that $x+(-1)x=0$, showing that the additive inverse of $x$ is
simply the product of $x$ with the additive inverse of $1$. By the definition
of $1$, the left-hand side of the above is equivalent to $(1)x+(-1)x$. Then,
using the 9th property of a commutative ring, we can say
\[
(1)x+(-1)x=(1+(-1))x=0x=0
\]
Thus, $-x$ is indeed the additive inverse.

\textbf{(b) Let $\phi:R\to R$ be defined by $\phi(x) = -x$. Prove that $\phi$ is
a homomorphism if and only if $1 + 1 = 0$ in $R$.}

Suppose $\phi$ is a homomorphism. Then, by definition of a homomorphism,
$\phi(1)=1$. But, by the definition of $\phi$, $\phi(1)=-1$. In order for this
to be possible, $-1$ must be the same as $1$; so $1=-1$. Adding $1$ to both
sides we get $1+1=-1+1=0$, so the condition is necessary.

To show it is sufficient, we assume $1+1=0$ and show that the definition of a
homomorphism is met. Firstly, it is clear that
$\phi(r_1+r_2)=-(r_1+r_2)=(-1)(r_1+r_2)=-r_1-r_2=\phi(r_1)+\phi(r_2)$.
Similarly, $\phi(r_1r_2)=-r_1r_2=(-1)r_1(1)r_2$. But, since $1+1=0$, we we can
subtract $1$ from both sides to get $1=-1$, so the previous expression is
equivalent to $(-1)r_1(-1)r_2=\phi(r_1)\phi(r_2)$, so $\phi$ is also closed
under multiplication. Lastly, we need to show that $\phi(1)=1$, but as we just
stated, $1=-1$, so $\phi(1)=-1=1$, and we are done.

\textbf{7. Suppose $\phi$ is a ring homomorphism from $\mathbb Z\times\mathbb Z$
to $\mathbb Z\times\mathbb Z$. What are the possibilities for $\phi((1,0))$?
Make sure you list all possible values of $\phi((1,0))$, and for each value give
an example of a homomorphism that acheives it.}

\textbf{8. Let $R$ be a commutative ring, and let $N\subseteq R$ be the set of
elements $x\in R$ such that $x^n=0$ for some positive integer $n$. Is $N$
necessarily an ideal of $R$? If yes, prove it. If no, find a specific ring $R$
such that $N$ is not an ideal.}

\end{document}